WIP

SporkProofs/ParReduce.lean
@@ -1,64 +1,40 @@
 import SporkProofs.Syntax
+import SporkProofs.Notation
 
--- start(): spork(body(), g())
--- body(): call f() ⊳ cont(·)
--- cont(x): spoin(unpr(x), prom(x, ·))
--- unpr(x): call g() ⊳ ret(x, ·)
--- prom(x, y): goto ret(x, y)
--- ret(x, y): return(x,y)
-
-def parSSA : Function [⟨0,1⟩, ⟨0,1⟩, ⟨0,2⟩] ⟨0,2⟩ :=
-  let f : Var 3 := 0
-  let g : Var 3 := 1
+def parSSA (f g : FuncIdx): Func :=
   func (
-    bb start() {SPORK 1 (goto body(), g())},
-    bb body() sporks (1) {CALL f() ⊳ goto cont()},
-    bb cont(x) sporks (1) {SPOIN (goto unpr(x), goto prom(x))},
-    bb unpr(x) {CALL g() ⊳ goto ret(x)},
-    bb prom(x, y) {GOTO ret(x,y)},
-    bb ret(x, y) {RETURN(x, y)}
+    block start() {SPORK (goto body(), g())},
+    block body() sporks (1) {CALL f() ⊳ goto cont()},
+    block cont(x) sporks (1) {SPOIN (goto unpr(x), goto prom(x))},
+    block unpr(x) {CALL g() ⊳ goto ret(x)},
+    block prom(x, y) {GOTO ret(x,y)},
+    block ret(x, y) {RETURN(x, y)}
   )
 
--- reduce(z,a,i,j) -> a₁
---   start(z,a,i,j): goto guard(z,i,j,a)
---   guard(z,i,j,a): b ← i ≥ j; if b then done(a) else iter(z,i,j,a)
---   done(a): return(a)
---   iter(z,i,j,a): spork(body(z,i,j,a), split(z,i,j,a))
---   body(z,i,j,a): call f(i) ⊳ accum(z,i,j,a,·)
---   accum(z,i,j,a,a₁): call c(a,a₁) ⊳ cont(z,i,j,·)
---   cont(z,i,j,a): spoin(next(z,i,j,a), break(a,·))
---   next(z,i,j,a): i₁ ← i + 1; goto guard(z,i₁,j,a)
---   break(a,a₁): call c(a,a₁) ⊳ done(·)
-
--- split(z,a,i,j) -> a₁
---   spwn(z,a,i,j): i₁ ← i + 1; k ← i₁ + j; m ← k / 2; spork(left(z,i₁,m), reduce(z,z,m,j))
---   left(z,i,m): call reduce(z,z,i,m) ⊳ middle(z,m,j,·)
---   middle(z,m,j,a): spoin(leftover(z,m,j,a), join(a,·))
---   leftover(z,m,j,a): call reduce(z,a,m,j) ⊳ exit(·)
---   join(a,a₁): call c(a,a₁) ⊳ exit(·)
---   exit(a): return(a)
-
-def redSSA : Function [⟨2,1⟩, ⟨1,1⟩, ⟨4,1⟩, ⟨4,1⟩] ⟨4,1⟩ × Function [⟨2,1⟩, ⟨1,1⟩, ⟨4,1⟩, ⟨4,1⟩] ⟨4,1⟩ :=
-  let     c : Var 4 := 0
-  let     f : Var 4 := 1
-  let   red : Var 4 := 2
-  let split : Var 4 := 3
+def redSSA (c f red split : FuncIdx) : Func × Func :=
   (func (
-     bb start(z,a,i,j) {GOTO guard(z,i,j,a)},
-     bb guard(z,i,j,a) {b ← i >= j, IF b THEN goto done(a) ELSE goto iter(z,i,j,a)},
-     bb done(a) {RETURN(a)},
-     bb iter(z,i,j,a) {SPORK 1 (goto body(z,i,j,a), split(z,i,j,a))},
-     bb body(z,i,j,a) sporks (1) {CALL f(i) ⊳ goto accum(z,i,j,a)},
-     bb accum(z,i,j,a,a₁) sporks (1) {CALL c(a,a₁) ⊳ goto cont(z,i,j)},
-     bb cont(z,i,j,a) sporks (1) {SPOIN (goto next(z,i,j,a), goto brk(a))},
-     bb next(z,i,j,a) {i₁ ← i + 1, GOTO guard(z,i₁,j,a)},
-     bb brk(a,a₁) {CALL c(a,a₁) ⊳ goto done()}
+     block start(z,a,i,j) {GOTO guard(z,i,j,a)},
+     block guard(z,i,j,a) {b ← i >= j, IF b THEN goto done(a) ELSE goto iter(z,i,j,a)},
+     block done(a) {RETURN(a)},
+     block iter(z,i,j,a) {SPORK (goto body(z,i,j,a), split(z,i,j,a))},
+     block body(z,i,j,a) sporks (1) {CALL f(i) ⊳ goto accum(z,i,j,a)},
+     block accum(z,i,j,a,a₁) sporks (1) {CALL c(a,a₁) ⊳ goto cont(z,i,j)},
+     block cont(z,i,j,a) sporks (1) {SPOIN (goto next(z,i,j,a), goto brk(a))},
+     block next(z,i,j,a) {i₁ ← i + 1, GOTO guard(z,i₁,j,a)},
+     block brk(a,a₁) {CALL c(a,a₁) ⊳ goto done()}
    ),
    func (
-     bb spwn(z,a,i,j) {i₁ ← i + 1, k ← i₁ + j, m ← k / 2, SPORK 1 (goto left(z,i₁,m,j), red(z,z,m,j))},
-     bb left(z,i,m,j) sporks (1) {CALL red(z,z,i,m) ⊳ goto middle(z,m,j)},
-     bb middle(z,m,j,a) sporks (1) {SPOIN(goto leftover(z,m,j,a), goto join(a))},
-     bb leftover(z,m,j,a) {CALL red(z,a,m,j) ⊳ goto exit()},
-     bb join(a,a₁) {CALL c(a,a₁) ⊳ goto exit()},
-     bb exit(a) {RETURN(a)}
+     block spwn(z,a,i,j) {i₁ ← i + 1, k ← i₁ + j, m ← k / 2, SPORK (goto left(z,i₁,m,j), red(z,z,m,j))},
+     block left(z,i,m,j) sporks (1) {CALL red(z,z,i,m) ⊳ goto middle(z,m,j)},
+     block middle(z,m,j,a) sporks (1) {SPOIN(goto leftover(z,m,j,a), goto join(a))},
+     block leftover(z,m,j,a) {CALL red(z,a,m,j) ⊳ goto exit()},
+     block join(a,a₁) {CALL c(a,a₁) ⊳ goto exit()},
+     block exit(a) {RETURN(a)}
    ))  
+
+theorem parSSAOkay : (parSSA 0 1).Okay [FuncSig.mk 0 1, FuncSig.mk 0 1] :=
+  by trivial
+theorem redSSAOkay :
+    let fsigs := [FuncSig.mk 2 1, FuncSig.mk 1 1, FuncSig.mk 4 1, FuncSig.mk 4 1]
+    (redSSA 0 1 2 3).fst.Okay fsigs ∧ (redSSA 0 1 2 3).snd.Okay fsigs :=
+  by trivial
