SporkProofs/Syntax.lean
@@ -1,61 +1,5 @@
 --import Mathlib.Tactic.Linarith
-
-inductive IVec {α : Type} (β : α -> Sort) : List α -> Sort where
-  | nil : IVec β []
-  | cons : {h : α} -> {t : List α} -> β h -> IVec β t -> IVec β (h :: t)
-
-namespace IVec
-  /--
-    get the jth index in an ivec
-  -/
-  def get {α : Type} {β : α -> Sort} {l : List α} : IVec β l -> (j : Fin l.length) -> β l[j]
-    | cons h' _, ⟨0, _⟩ => h'
-    | cons _ t', ⟨Nat.succ j, pj⟩ => get t' ⟨j, Nat.lt_of_succ_lt_succ pj⟩
-
-  @[inherit_doc get]
-  syntax:max term noWs "⁅" withoutPosition(term) "⁆" : term
-  macro_rules | `($x⁅$i⁆) => `(($x).get (Fin.mk $i (by get_elem_tactic)))
-
-  def head {α : Type} {β : α -> Sort} {l : List α} :
-           (v : IVec β l) -> (p : l ≠ []) -> β (l.head p)
-    | cons h _t, _p => h
-
-  def head' {α : Type} {β : α -> Sort} {a : α} {l : List α} :
-           (v : IVec β (a :: l)) -> β a
-    | cons h _t => h
-
-  def tail {α : Type} {β : α -> Sort} {l : List α} :
-           IVec β l -> IVec β l.tail
-    | nil => nil
-    | cons _h t => t
-
-  def map {α α' : Type} {β : α -> Sort} : {l : List α} -> ((a : α) -> β a -> α') -> IVec β l -> List α'
-    | [], _f, _n => []
-    | a :: _as, f, v => f a (head' v) :: v.tail.map f
-
-  theorem map_length {α α' : Type} {β : α -> Sort} : {l : List α} -> (f : (a : α) -> β a -> α') -> (v : IVec β l) -> (l.length = (v.map f).length)
-    | [], _f, _n => rfl
-    | a :: as, f, cons v vs => by simp; exact map_length f vs ▸ rfl
-
-  instance instDecidable {α : Type} {β : α -> Prop} [DecidablePred β] : {l : List α} -> Decidable (IVec β l)
-    | [] => isTrue nil
-    | a :: as =>
-      let _ : Decidable (IVec β as) := instDecidable
-      dite (β a)
-        (decidable_of_iff (IVec β as) ⟨cons ·, tail⟩)
-        (isFalse ∘ λ f (.cons h _t) => f h)
-
-  def append {α β} : {l l' : List α} -> IVec β l -> IVec β l' -> IVec β (l ++ l')
-    | [], _bs, nil, ws => ws
-    | _a :: _as, _bs, cons v vs, ws => cons v (append vs ws)
-
-  def unappend {α : Type} {β : α -> Sort} :
-           {l l' : List α} -> IVec β (l ++ l') -> IVec β l ×' IVec β l'
-    | [], _l', xs => ⟨nil, xs⟩
-    | _a :: _l, _l', v => let ⟨v1, v2⟩ := unappend v.tail; ⟨cons v.head' v1, v2⟩
-
-  def singleton {α β} {a : α} (b : β a) : IVec β [a] := nil.cons b
-end IVec
+import SporkProofs.IVec
 
 abbrev Val := Int
 
@@ -126,22 +70,24 @@ namespace BlockSig
   abbrev spork | mk a ss, s => mk a (s :: ss)
   abbrev spoin | mk a ss => mk a ss.tail
 
-  instance instDecidableEq : DecidableEq BlockSig
-    | ⟨ar, sn⟩, ⟨ar', sn'⟩ =>
-        decidable_of_iff ((ar, sn) = (ar', sn'))
-          ⟨congrArg (λ (areq, sneq) => mk areq sneq),
-           congrArg (λ | mk areq sneq => (areq, sneq))⟩
+  -- instance instDecidableEq : DecidableEq BlockSig
+  --   | ⟨ar, sn⟩, ⟨ar', sn'⟩ =>
+  --       decidable_of_iff ((ar, sn) = (ar', sn'))
+  --         ⟨congrArg (λ (areq, sneq) => mk areq sneq),
+  --          congrArg (λ | mk areq sneq => (areq, sneq))⟩
+  deriving instance DecidableEq for BlockSig
 end BlockSig
 
 namespace FuncSig
   abbrev arity | mk a _r => a
   abbrev ret | mk _a r => r
 
-  instance instDecidableEq : DecidableEq FuncSig
-    | ⟨arity, ret⟩, ⟨arity', ret'⟩ =>
-      decidable_of_iff ((arity, ret) = (arity', ret'))
-        ⟨congrArg (λ (areq, sneq) => mk areq sneq),
-         congrArg (λ | mk areq sneq => (areq, sneq))⟩
+  -- instance instDecidableEq : DecidableEq FuncSig
+  --   | ⟨arity, ret⟩, ⟨arity', ret'⟩ =>
+  --     decidable_of_iff ((arity, ret) = (arity', ret'))
+  --       ⟨congrArg (λ (areq, sneq) => mk areq sneq),
+  --        congrArg (λ | mk areq sneq => (areq, sneq))⟩
+  deriving instance DecidableEq, Inhabited for FuncSig
 end FuncSig
 
 namespace Var
@@ -155,8 +101,16 @@ namespace Var
   instance instDecidable (v : Var) : Decidable (v.Okay Γ) :=
     decidable_of_iff (v.idx < Γ) ⟨(⟨·⟩), (·.1)⟩
   
-  instance instDecidableEq : DecidableEq Var
-    | ⟨v⟩, ⟨v'⟩ => decidable_of_iff (v = v') ⟨congrArg mk, λ eq => congrArg (·.1) eq⟩
+  -- instance instDecidableEq : DecidableEq Var
+  --   | ⟨v⟩, ⟨v'⟩ => decidable_of_iff (v = v') ⟨congrArg mk, λ eq => congrArg (·.1) eq⟩
+  deriving instance DecidableEq for Var
+
+  instance instOfNat {n} : OfNat Var n where
+    ofNat := Var.mk n
+  instance instCoeVarToNat : Coe Nat Var where
+    coe := mk
+  instance instCoeNatToVar : Coe Var Nat where
+    coe := idx
 end Var
 
 namespace Atom
@@ -170,25 +124,28 @@ namespace Atom
     | val _v => isTrue Okay.val
     | var v => decidable_of_iff (v.Okay Γ) ⟨Okay.var, λ (.var v) => v⟩
 
-  instance instDecidableEq : DecidableEq Atom
-    | val v, val v' => decidable_of_iff (v = v')
-        ⟨congrArg val, λ eq => congrArg (λ | (val v) => v | _ => v) eq⟩
-    | var v, var v' => decidable_of_iff (v = v')
-        ⟨congrArg var, λ eq => congrArg (λ | (var v) => v | _ => v) eq⟩
-    | val v, var v' => isFalse (by simp)
-    | var v, val v' => isFalse (by simp)
+  -- instance instDecidableEq : DecidableEq Atom
+  --   | val v, val v' => decidable_of_iff (v = v')
+  --       ⟨congrArg val, λ eq => congrArg (λ | (val v) => v | _ => v) eq⟩
+  --   | var v, var v' => decidable_of_iff (v = v')
+  --       ⟨congrArg var, λ eq => congrArg (λ | (var v) => v | _ => v) eq⟩
+  --   | val v, var v' => isFalse (by simp)
+  --   | var v, val v' => isFalse (by simp)
+  deriving instance DecidableEq for Atom
 end Atom
 
 namespace Uop
-  instance instDecidableEq : DecidableEq Uop
-    | a, b => by cases a <;> cases b <;>
-                 first | exact isTrue rfl | exact isFalse (by simp)
+  -- instance instDecidableEq : DecidableEq Uop
+  --   | a, b => by cases a <;> cases b <;>
+  --                first | exact isTrue rfl | exact isFalse (by simp)
+  deriving instance DecidableEq for Uop
 end Uop
 
 namespace Bop
-  instance instDecidableEq : DecidableEq Bop
-    | a, b => by cases a <;> cases b <;>
-                 first | exact isTrue rfl | exact isFalse (by simp)
+  -- instance instDecidableEq : DecidableEq Bop
+  --   | a, b => by cases a <;> cases b <;>
+  --                first | exact isTrue rfl | exact isFalse (by simp)
+  deriving instance DecidableEq for Bop
 end Bop
 
 namespace Expr
@@ -207,25 +164,26 @@ namespace Expr
     | bop _o a b => decidable_of_iff (a.Okay Γ ∧ b.Okay Γ)
         ⟨And.elim Okay.bop, λ (.bop a b) => ⟨a, b⟩⟩
 
-  instance instDecidableEq : DecidableEq Expr
-    | nop v, nop v' =>
-      decidable_of_iff (v = v')
-        ⟨congrArg nop,
-         congrArg (λ | nop v => v | _ => v)⟩
-    | uop o a, uop o' a' =>
-      decidable_of_iff ((o, a) = (o', a'))
-        ⟨congrArg (λ (o, a) => uop o a),
-         congrArg (λ | uop o a => (o, a) | _ => (o, a))⟩
-    | bop o a b, bop o' a' b' =>
-      decidable_of_iff ((o, a, b) = (o', a', b'))
-        ⟨congrArg (λ (o, a, b) => bop o a b),
-         congrArg (λ | bop o a b => (o, a, b) | _ => (o, a, b))⟩
-    | nop _, uop _ _ => isFalse (by simp)
-    | nop _, bop _ _ _ => isFalse (by simp)
-    | uop _ _, nop _ => isFalse (by simp)
-    | uop _ _, bop _ _ _ => isFalse (by simp)
-    | bop _ _ _, nop _ => isFalse (by simp)
-    | bop _ _ _, uop _ _ => isFalse (by simp)
+  -- instance instDecidableEq : DecidableEq Expr
+  --   | nop v, nop v' =>
+  --     decidable_of_iff (v = v')
+  --       ⟨congrArg nop,
+  --        congrArg (λ | nop v => v | _ => v)⟩
+  --   | uop o a, uop o' a' =>
+  --     decidable_of_iff ((o, a) = (o', a'))
+  --       ⟨congrArg (λ (o, a) => uop o a),
+  --        congrArg (λ | uop o a => (o, a) | _ => (o, a))⟩
+  --   | bop o a b, bop o' a' b' =>
+  --     decidable_of_iff ((o, a, b) = (o', a', b'))
+  --       ⟨congrArg (λ (o, a, b) => bop o a b),
+  --        congrArg (λ | bop o a b => (o, a, b) | _ => (o, a, b))⟩
+  --   | nop _, uop _ _ => isFalse (by simp)
+  --   | nop _, bop _ _ _ => isFalse (by simp)
+  --   | uop _ _, nop _ => isFalse (by simp)
+  --   | uop _ _, bop _ _ _ => isFalse (by simp)
+  --   | bop _ _ _, nop _ => isFalse (by simp)
+  --   | bop _ _ _, uop _ _ => isFalse (by simp)
+  deriving instance DecidableEq for Expr
 end Expr
 
 namespace Cont
@@ -280,11 +238,12 @@ namespace Cont
   instance instDecidable (b : Cont) : Decidable (b.Okay bsigs bsig) :=
     decidable_of_iff (b.OkayRets bsigs bsig 0) OkayRets0_iff_Okay
 
-  instance instDecidableEq : DecidableEq Cont
-    | ⟨b, args⟩, ⟨b', args'⟩ => decidable_of_iff
-        ((b, args) = (b', args'))
-        ⟨congrArg (λ (b, args) => mk b args),
-         congrArg (λ | mk b args => (b, args))⟩
+  -- instance instDecidableEq : DecidableEq Cont
+  --   | ⟨b, args⟩, ⟨b', args'⟩ => decidable_of_iff
+  --       ((b, args) = (b', args'))
+  --       ⟨congrArg (λ (b, args) => mk b args),
+  --        congrArg (λ | mk b args => (b, args))⟩
+  deriving instance DecidableEq for Cont
 end Cont
 
 namespace Transfer
@@ -379,44 +338,45 @@ namespace Transfer
               ⟨λ ⟨a, b⟩ => Okay.spoin (by simp) a b,
                λ | .spoin h' a b => ⟨a, b⟩⟩
 
-  instance instDecidableEq : DecidableEq Transfer
-    | t, t' => by
-      cases t <;> cases t' <;>
+  -- instance instDecidableEq : DecidableEq Transfer
+  --   | t, t' => by
+  --     cases t <;> cases t' <;>
 
-      -- for mismatched constructors, automatically
-      -- derive isFalse by contradiction:
-      try (apply isFalse; intro; contradiction)
+  --     -- for mismatched constructors, automatically
+  --     -- derive isFalse by contradiction:
+  --     try (apply isFalse; intro; contradiction)
 
-      -- remaining cases, potentially isTrue:
-      · case goto.goto bnext bnext' =>
-          exact decidable_of_iff (bnext = bnext')
-            ⟨congrArg goto,
-             congrArg (λ | goto bnext => bnext | _ => bnext)⟩
+  --     -- remaining cases, potentially isTrue:
+  --     · case goto.goto bnext bnext' =>
+  --         exact decidable_of_iff (bnext = bnext')
+  --           ⟨congrArg goto,
+  --            congrArg (λ | goto bnext => bnext | _ => bnext)⟩
 
-      · case ite.ite cond bthen belse cond' bthen' belse' =>
-          exact decidable_of_iff ((cond, bthen, belse) = (cond', bthen', belse'))
-            ⟨congrArg (λ (a, b, c) => ite a b c),
-             congrArg (λ | ite a b c => (a, b, c) | _ => (cond, bthen, belse))⟩
+  --     · case ite.ite cond bthen belse cond' bthen' belse' =>
+  --         exact decidable_of_iff ((cond, bthen, belse) = (cond', bthen', belse'))
+  --           ⟨congrArg (λ (a, b, c) => ite a b c),
+  --            congrArg (λ | ite a b c => (a, b, c) | _ => (cond, bthen, belse))⟩
 
-      · case call.call f args bret f' args' bret' =>
-          exact decidable_of_iff ((f, args, bret) = (f', args', bret'))
-            ⟨congrArg (λ (a, b, c) => call a b c),
-             congrArg (λ | call f args bret => (f, args, bret) | _ => (f, args, bret))⟩
+  --     · case call.call f args bret f' args' bret' =>
+  --         exact decidable_of_iff ((f, args, bret) = (f', args', bret'))
+  --           ⟨congrArg (λ (a, b, c) => call a b c),
+  --            congrArg (λ | call f args bret => (f, args, bret) | _ => (f, args, bret))⟩
 
-      · case retn.retn args args' =>
-          exact decidable_of_iff (args = args')
-            ⟨congrArg retn,
-             congrArg (λ | retn args => args | _ => args)⟩
+  --     · case retn.retn args args' =>
+  --         exact decidable_of_iff (args = args')
+  --           ⟨congrArg retn,
+  --            congrArg (λ | retn args => args | _ => args)⟩
 
-      · case spork.spork bbody fspwn args bbody' fspwn' args' =>
-          exact decidable_of_iff ((bbody, fspwn, args) = (bbody', fspwn', args'))
-            ⟨congrArg (λ (a, b, c) => spork a b c),
-             congrArg (λ | spork a b c => (a, b, c) | _ => (bbody, fspwn, args))⟩
+  --     · case spork.spork bbody fspwn args bbody' fspwn' args' =>
+  --         exact decidable_of_iff ((bbody, fspwn, args) = (bbody', fspwn', args'))
+  --           ⟨congrArg (λ (a, b, c) => spork a b c),
+  --            congrArg (λ | spork a b c => (a, b, c) | _ => (bbody, fspwn, args))⟩
 
-      · case spoin.spoin bunpr bprom bunpr' bprom' =>
-          exact decidable_of_iff ((bunpr, bprom) = (bunpr', bprom'))
-            ⟨congrArg (λ (a, b) => spoin a b),
-             congrArg (λ | spoin a b => (a, b) | _ => (bunpr, bprom))⟩
+  --     · case spoin.spoin bunpr bprom bunpr' bprom' =>
+  --         exact decidable_of_iff ((bunpr, bprom) = (bunpr', bprom'))
+  --           ⟨congrArg (λ (a, b) => spoin a b),
+  --            congrArg (λ | spoin a b => (a, b) | _ => (bunpr, bprom))⟩
+  deriving instance DecidableEq for Transfer
 end Transfer
 
 namespace Code
@@ -424,6 +384,10 @@ namespace Code
     (fsigs : FuncSigs)
     (bsigs : BlockSigs)
     (ret : Nat)
+
+  abbrev view : Code -> List Expr × Transfer
+    | stmt e c => let (es, t) := view c; (e :: es, t)
+    | trfr t => ([], t)
 
   inductive Okay : (bsig : BlockSig) -> Code -> Prop where
     | stmt
@@ -459,18 +423,19 @@ namespace Code
         ⟨Okay.trfr,
          λ | Okay.trfr a => a⟩
 
-  instance instDecidableEq : DecidableEq Code
-    | stmt e c, stmt e' c' =>
-      let _ : Decidable (c = c') := instDecidableEq c c'
-      decidable_of_iff (e = e' ∧ c = c')
-      ⟨λ ⟨a, b⟩ => a ▸ b ▸ rfl,
-       λ p => ⟨congrArg (λ | stmt e c => e | _ => e) p,
-               congrArg (λ | stmt e c => c | _ => c) p⟩⟩
-    | trfr t, trfr t' => decidable_of_iff (t = t')
-        ⟨congrArg trfr,
-         congrArg (λ | trfr t => t | _ => t)⟩
-    | stmt _ _, trfr _ => isFalse (by simp)
-    | trfr _, stmt _ _ => isFalse (by simp)
+  -- instance instDecidableEq : DecidableEq Code
+  --   | stmt e c, stmt e' c' =>
+  --     let _ : Decidable (c = c') := instDecidableEq c c'
+  --     decidable_of_iff (e = e' ∧ c = c')
+  --     ⟨λ ⟨a, b⟩ => a ▸ b ▸ rfl,
+  --      λ p => ⟨congrArg (λ | stmt e c => e | _ => e) p,
+  --              congrArg (λ | stmt e c => c | _ => c) p⟩⟩
+  --   | trfr t, trfr t' => decidable_of_iff (t = t')
+  --       ⟨congrArg trfr,
+  --        congrArg (λ | trfr t => t | _ => t)⟩
+  --   | stmt _ _, trfr _ => isFalse (by simp)
+  --   | trfr _, stmt _ _ => isFalse (by simp)
+  deriving instance DecidableEq for Code
 end Code
 
 namespace Block
@@ -490,11 +455,13 @@ namespace Block
       decidable_of_iff (code.Okay fsigs bsigs ret bsig)
         ⟨λ a => .mk a, λ | .mk a => a⟩
 
-  instance instDecidableEq : DecidableEq Block
-    | mk bsig code, mk bsig' code' =>
-      decidable_of_iff ((bsig, code) = (bsig', code'))
-        ⟨congrArg (λ (a, b) => mk a b),
-         λ x => congrArg (λ | .mk a b => (a, b)) x⟩
+  -- instance instDecidableEq : DecidableEq Block
+  --   | mk bsig code, mk bsig' code' =>
+  --     decidable_of_iff ((bsig, code) = (bsig', code'))
+  --       ⟨congrArg (λ (a, b) => mk a b),
+  --        λ x => congrArg (λ | .mk a b => (a, b)) x⟩
+
+  deriving instance DecidableEq for Block
 
   instance instInhabited : Inhabited Block where
     default := mk ⟨0, []⟩ (Code.trfr (Transfer.retn []))
@@ -542,11 +509,12 @@ namespace Func
          HeadIs blocks (·.bsig) ⟨fsig.arity, []⟩)
         ⟨λ ⟨a, b⟩ => Okay.mk a b, λ | .mk a b => ⟨a, b⟩⟩
 
-  instance instDecidableEq : DecidableEq Func
-    | mk fsig blocks, mk fsig' blocks' =>
-      decidable_of_iff ((fsig, blocks) = (fsig', blocks'))
-        ⟨congrArg (λ (a, b) => mk a b),
-         λ x => congrArg (λ | .mk a b => (a, b)) x⟩
+  -- instance instDecidableEq : DecidableEq Func
+  --   | mk fsig blocks, mk fsig' blocks' =>
+  --     decidable_of_iff ((fsig, blocks) = (fsig', blocks'))
+  --       ⟨congrArg (λ (a, b) => mk a b),
+  --        λ x => congrArg (λ | .mk a b => (a, b)) x⟩
+  deriving instance DecidableEq for Func
 
   instance instInhabited : Inhabited Func where
     default := mk ⟨0, 0⟩ default
@@ -570,165 +538,10 @@ namespace Program
          HeadIs funs (·.fsig) ⟨0, 1⟩)
         ⟨λ ⟨a, b⟩ => Okay.mk a b, λ | .mk a b => ⟨a, b⟩⟩
 
-  instance instDecidableEq : DecidableEq Program
-    | mk funs, mk funs' =>
-      decidable_of_iff (funs = funs')
-        ⟨congrArg mk, λ x => congrArg (λ | .mk a => a) x⟩
+  -- instance instDecidableEq : DecidableEq Program
+  --   | mk funs, mk funs' =>
+  --     decidable_of_iff (funs = funs')
+  --       ⟨congrArg mk, λ x => congrArg (λ | .mk a => a) x⟩
+  deriving instance DecidableEq for Program
 end Program
 
-
-/- TODO: will need to revisit this
-section macros
-  open Lean Elab Command Term Macro
-
-  declare_syntax_cat ssa_atom
-  declare_syntax_cat ssa_unaop
-  declare_syntax_cat ssa_binop
-  declare_syntax_cat ssa_expr
-  declare_syntax_cat stmtget
-  declare_syntax_cat BB
-
-  syntax "var" "⟨" term "⟩" : term
-  syntax "vec" "⟨" term,* "⟩" : term
-  syntax "ivec" "⟨" term,* "⟩" : term
-  syntax "list?" "[" term,* "]" : term
-  syntax (name := goto) "goto " term:max "(" term,* ")" : term
-  syntax (name := GOTO) "GOTO " term:max "(" term,* ")" : term
-  syntax (name := CALL) "CALL " term:max "(" term,* ")" "⊳" term : term
-  syntax (name := RETURN) "RETURN " "(" term,* ")" : term
-  syntax (name := SPORK) "SPORK " term:max "(" term "," term:max "(" term,* ")" ")" : term
-  syntax (name := SPOIN) "SPOIN " "(" term "," term ")" : term
-  syntax (name := ITE) "IF " ssa_atom " THEN " term " ELSE " term : term
-  syntax num : ssa_atom
-  syntax ident : ssa_atom
-  syntax "¬" : ssa_unaop
-  syntax "-" : ssa_unaop
-  syntax "+" : ssa_binop
-  syntax "-" : ssa_binop
-  syntax "*" : ssa_binop
-  syntax "/" : ssa_binop
-  syntax "%" : ssa_binop
-  syntax "<" : ssa_binop
-  syntax "≤" : ssa_binop
-  syntax "<=" : ssa_binop
-  syntax ">" : ssa_binop
-  syntax "≥" : ssa_binop
-  syntax ">=" : ssa_binop
-  syntax "==" : ssa_binop
-  syntax "!=" : ssa_binop
-  syntax "&&" : ssa_binop
-  syntax "||" : ssa_binop
-  syntax "^^" : ssa_binop
-  syntax ssa_atom : ssa_expr
-  syntax ssa_unaop ssa_atom : ssa_expr
-  syntax ssa_atom ssa_binop ssa_atom : ssa_expr
-  syntax "[expr| " ssa_expr " ]" : term
-  syntax "stmts " num "{" stmtget "}" : term
-  syntax term : stmtget
-  syntax ident " ← " ssa_expr "," stmtget : stmtget
-  syntax (name := countIdents) "countIdents " ident* : term
-  syntax (name := blocklets') "blocklets' " ident,* " from " num " to " term " in " term : term
-  syntax "bb " ident "(" ident,* ")" ("sporks " "(" term,* ")")? "{" stmtget "}" : BB
-  syntax "func" "(" BB,* ")" : term
-  syntax "blocksh" "⟨" BB* "⟩" "⟨" ident* "⟩" "⟨" term:max* "⟩" "⟨" term:max* "⟩" : term
-
-  def elabSSAAtom : Macro
-    | `(ssa_atom| $n:num) => `(Atom.val ($n))
-    | `(ssa_atom| $x:ident) => `(Atom.var ($x))
-    | _ => Macro.throwUnsupported
-  
-  def elabSSAUnaOp : Macro
-    | `(ssa_unaop| -) => `(Uop.INEG)
-    | `(ssa_unaop| ¬) => `(Uop.LNOT)
-    | _ => Macro.throwUnsupported
-  
-  def elabSSABinOp : Macro
-    | `(ssa_binop| +)  => `(Bop.IADD)
-    | `(ssa_binop| -)  => `(Bop.ISUB)
-    | `(ssa_binop| *)  => `(Bop.IMUL)
-    | `(ssa_binop| /)  => `(Bop.IDIV)
-    | `(ssa_binop| %)  => `(Bop.IMOD)
-    | `(ssa_binop| <)  => `(Bop.ILT)
-    | `(ssa_binop| <=) => `(Bop.ILE)
-    | `(ssa_binop| ≤)  => `(Bop.ILE)
-    | `(ssa_binop| >)  => `(Bop.IGT)
-    | `(ssa_binop| >=) => `(Bop.IGE)
-    | `(ssa_binop| ≥)  => `(Bop.IGE)
-    | `(ssa_binop| ==) => `(Bop.IEQ)
-    | `(ssa_binop| !=) => `(Bop.INE)
-    | `(ssa_binop| &&) => `(Bop.LAND)
-    | `(ssa_binop| ||) => `(Bop.LOR)
-    | `(ssa_binop| ^^) => `(Bop.LXOR)
-    | _ => Macro.throwUnsupported
-
-  macro_rules
-    | `(var⟨$x⟩) => `(⟨$x, by first | decide | (norm_num; get_elem_tactic) | linarith⟩)
-
-    -- if only one element, first try to use that element
-    -- as the list itself, otherwise a singleton
-    -- this parses both list?[1,2,3] and list?[x] for some list x
-    | `(list?[$x:term]) => `(by first | exact [($x)] | exact ($x))
-    | `(list?[$xs,*]) => `([$xs,*])
-
-    -- | `(vec⟨$xs,*⟩) => `(⟨[$xs,*], rfl⟩)
-    | `(vec⟨$xs,*⟩) => `(⟨[$xs,*], (by first | rfl | simp)⟩)
-
-    | `(ivec⟨⟩) => `(IVec.nil)
-    | `(ivec⟨$x⟩) => `(IVec.cons ($x) IVec.nil)
-    | `(ivec⟨$x, $xs,*⟩) => `(IVec.cons ($x) (ivec⟨$xs,*⟩))
-
-    | `(goto $b ($args,*)) => `(Cont.mk ($b) [$args,*] (by first | rfl | simp))
-
-    | `(CALL $f ($args,*) ⊳ $cont) => `(Transfer.call ($f) vec⟨$args,*⟩ ($cont))
-    | `(RETURN ($args,*)) => `(Transfer.retn vec⟨$args,*⟩)
-    | `(GOTO $b ($args,*)) => `(Transfer.goto (goto $b ($args,*)))
-    | `(SPORK $sp ($body, $f ($args,*) ) ) => `(Transfer.spork ($sp) ($body) ($f) vec⟨$args,*⟩)
-    | `(SPOIN ($unpr, $prom)) => `(Transfer.spoin ($unpr) ($prom))
-    | `(IF $cond THEN $tt ELSE $ff) =>
-        elabSSAAtom cond >>= λ cond' =>
-        `(Transfer.ite ($(⟨cond'⟩)) ($tt) ($ff))
-
-    | `(ssa_expr| $a:ssa_atom) =>
-        elabSSAAtom a >>= λ a' =>
-        `(Expr.val ($(⟨a'⟩)))
-    | `(ssa_expr| $o:ssa_unaop $a:ssa_atom) =>
-        elabSSAUnaOp o >>= λ o' =>
-        elabSSAAtom a >>= λ a' =>
-        `(Expr.una ($(⟨o'⟩)) ($(⟨a'⟩)))
-    | `(ssa_expr| $a:ssa_atom $o:ssa_binop $b:ssa_atom) =>
-        elabSSABinOp o >>= λ o' =>
-        elabSSAAtom a >>= λ a' =>
-        elabSSAAtom b >>= λ b' =>
-        `(Expr.bin ($(⟨o'⟩)) ($(⟨a'⟩)) ($(⟨b'⟩)))
-
-    | `([expr| $se:ssa_expr ]) => `($(⟨se.1⟩))
-  
-    | `(stmts $_ { $t:term }) => `(trfr ($t))
-    | `(stmts $i { $x:ident ← $t:ssa_expr, $s:stmtget }) =>
-        let n := Syntax.mkNatLit (i.getNat + 1)
-        `(stmt ([expr|$t]) (let $x : Var ($n) := var⟨$i⟩; stmts $n { $s }))
-  
-    | `(countIdents $ids:ident*) =>
-        let n := ids.size
-        return Syntax.mkNatLit n
-
-    | `(blocklets' from $_ to $_ in $t) => `($t)
-    | `(blocklets' $x from $i to $j in $t) => `(let $x : Var ($j) := var⟨($i)⟩; $t)
-    | `(blocklets' $x, $xs:ident,* from $i to $j in $t) =>
-      let i' := Syntax.mkNatLit i.getNat.succ
-      `(let $x : Var ($j) := var⟨($i)⟩; blocklets' $xs,* from $(i') to ($j) in $t)
-  
-    | `(blocksh ⟨ ⟩ ⟨$bns*⟩ ⟨$bss*⟩ ⟨$bts*⟩) =>
-        `(Select.mk ⟨[$bss,*], rfl⟩ (blocklets' $bns,* from 0 to (countIdents $bns*) in ivec⟨$bts,*⟩))
-  
-    | `(blocksh ⟨bb $bn ($args,*) {$cs} $bs*⟩ ⟨$bns*⟩ ⟨$bss*⟩ ⟨$bts*⟩) =>
-        let n := Syntax.mkNatLit (args.getElems.size)
-        `(blocksh ⟨$bs*⟩ ⟨$bns* $bn⟩ ⟨$bss* ⟨(countIdents $args*), []⟩⟩ ⟨$bts* (blocklets' $args,* from 0 to (countIdents $args*) in stmts $n {$cs})⟩)
-  
-    | `(blocksh ⟨bb $bn ($args,*) sporks ($ss,*) {$cs} $bs*⟩ ⟨$bns*⟩ ⟨$bss*⟩ ⟨$bts*⟩) =>
-        let n := Syntax.mkNatLit (args.getElems.size)
-        `(blocksh ⟨$bs*⟩ ⟨$bns* $bn⟩ ⟨$bss* ⟨(countIdents $args*), [$ss,*]⟩⟩ ⟨$bts* (blocklets' $args,* from 0 to (countIdents $args*) in stmts $n {$cs})⟩)
-  
-    | `(func ($bbs,*)) => `(blocksh ⟨$bbs*⟩ ⟨⟩ ⟨⟩ ⟨⟩)
-end macros
--/
