SporkProofs/IVec.lean
@@ -1,0 +1,56 @@
+inductive IVec {α : Type} (β : α -> Sort) : List α -> Sort where
+  | nil : IVec β []
+  | cons : {h : α} -> {t : List α} -> β h -> IVec β t -> IVec β (h :: t)
+
+namespace IVec
+  /--
+    get the jth index in an ivec
+  -/
+  def get {α : Type} {β : α -> Sort} {l : List α} : IVec β l -> (j : Fin l.length) -> β l[j]
+    | cons h' _, ⟨0, _⟩ => h'
+    | cons _ t', ⟨Nat.succ j, pj⟩ => get t' ⟨j, Nat.lt_of_succ_lt_succ pj⟩
+
+  @[inherit_doc get]
+  syntax:max term noWs "⁅" withoutPosition(term) "⁆" : term
+  macro_rules | `($x⁅$i⁆) => `(($x).get (Fin.mk $i (by get_elem_tactic)))
+
+  def head {α : Type} {β : α -> Sort} {l : List α} :
+           (v : IVec β l) -> (p : l ≠ []) -> β (l.head p)
+    | cons h _t, _p => h
+
+  def head' {α : Type} {β : α -> Sort} {a : α} {l : List α} :
+           (v : IVec β (a :: l)) -> β a
+    | cons h _t => h
+
+  def tail {α : Type} {β : α -> Sort} {l : List α} :
+           IVec β l -> IVec β l.tail
+    | nil => nil
+    | cons _h t => t
+
+  def map {α α' : Type} {β : α -> Sort} : {l : List α} -> ((a : α) -> β a -> α') -> IVec β l -> List α'
+    | [], _f, _n => []
+    | a :: _as, f, v => f a (head' v) :: v.tail.map f
+
+  theorem map_length {α α' : Type} {β : α -> Sort} : {l : List α} -> (f : (a : α) -> β a -> α') -> (v : IVec β l) -> (l.length = (v.map f).length)
+    | [], _f, _n => rfl
+    | a :: as, f, cons v vs => by simp; exact map_length f vs ▸ rfl
+
+  instance instDecidable {α : Type} {β : α -> Prop} [DecidablePred β] : {l : List α} -> Decidable (IVec β l)
+    | [] => isTrue nil
+    | a :: as =>
+      let _ : Decidable (IVec β as) := instDecidable
+      dite (β a)
+        (decidable_of_iff (IVec β as) ⟨cons ·, tail⟩)
+        (isFalse ∘ λ f (.cons h _t) => f h)
+
+  def append {α β} : {l l' : List α} -> IVec β l -> IVec β l' -> IVec β (l ++ l')
+    | [], _bs, nil, ws => ws
+    | _a :: _as, _bs, cons v vs, ws => cons v (append vs ws)
+
+  def unappend {α : Type} {β : α -> Sort} :
+           {l l' : List α} -> IVec β (l ++ l') -> IVec β l ×' IVec β l'
+    | [], _l', xs => ⟨nil, xs⟩
+    | _a :: _l, _l', v => let ⟨v1, v2⟩ := unappend v.tail; ⟨cons v.head' v1, v2⟩
+
+  def singleton {α β} {a : α} (b : β a) : IVec β [a] := nil.cons b
+end IVec
