SporkProofs/Notation.lean
@@ -1,0 +1,153 @@
+--import SporkProofs.IVec
+import SporkProofs.Syntax
+-- open Lean Elab Command Term Macro
+
+@[simp] abbrev mkfunc : List Block -> Func
+  | bs => Func.mk (FuncSig.mk (getarity bs) (getret bs)) bs
+  where
+    getarity : List Block -> Nat
+      | [] => panic "cannot infer signature of empty function!"
+      | .mk bsig _ :: _ => bsig.arity
+    getret : List Block -> Nat
+      | [] => panic "cannot infer signature of function because it has no return!"
+      | .mk _ code :: bs => match code.view.snd with
+        | Transfer.retn rs => rs.length
+        | _ => getret bs
+
+declare_syntax_cat ssa_atom
+declare_syntax_cat ssa_unaop
+declare_syntax_cat ssa_binop
+declare_syntax_cat ssa_expr
+declare_syntax_cat stmtget
+declare_syntax_cat BB
+declare_syntax_cat opt_spork_sig
+
+--syntax "var" "⟨" term "⟩" : term
+syntax "list?" "[" term,* "]" : term
+syntax (name := goto) "goto " term:max "(" term,* ")" : term
+syntax (name := GOTO) "GOTO " term:max "(" term,* ")" : term
+syntax (name := CALL) "CALL " term:max "(" term,* ")" "⊳" term : term
+syntax (name := RETURN) "RETURN " "(" term,* ")" : term
+syntax (name := SPORK) "SPORK " "(" term "," term:max "(" term,* ")" ")" : term
+syntax (name := SPOIN) "SPOIN " "(" term "," term ")" : term
+syntax (name := ITE) "IF " ssa_atom " THEN " term " ELSE " term : term
+syntax num : ssa_atom
+syntax ident : ssa_atom
+syntax "¬" : ssa_unaop
+syntax "-" : ssa_unaop
+syntax "+" : ssa_binop
+syntax "-" : ssa_binop
+syntax "*" : ssa_binop
+syntax "/" : ssa_binop
+syntax "%" : ssa_binop
+syntax "<" : ssa_binop
+syntax "≤" : ssa_binop
+syntax "<=" : ssa_binop
+syntax ">" : ssa_binop
+syntax "≥" : ssa_binop
+syntax ">=" : ssa_binop
+syntax "==" : ssa_binop
+syntax "!=" : ssa_binop
+syntax "&&" : ssa_binop
+syntax "||" : ssa_binop
+syntax "^^" : ssa_binop
+syntax ssa_atom : ssa_expr
+syntax ssa_unaop ssa_atom : ssa_expr
+syntax ssa_atom ssa_binop ssa_atom : ssa_expr
+syntax "[expr| " ssa_expr "]" : term
+syntax "stmts " num "{" stmtget "}" : term
+syntax term : stmtget
+syntax ident " ← " ssa_expr "," stmtget : stmtget
+syntax (name := countIdents) "countIdents " ident* : term
+syntax (name := blocklets) "blocklets " ident* " from " num " in " term : term
+syntax (name := somesporksig) ("sporks " "(" term,* ")")? : opt_spork_sig
+syntax "block " ident "(" ident,* ")" ("sporks " "(" term,* ")")? "{" stmtget "}" : BB
+syntax "func" "(" BB,* ")" : term
+syntax "blocksh" "⟨" BB* "⟩" "⟨" ident* "⟩" "⟨" term:max* "⟩" "⟨" term:max* "⟩" : term
+syntax "parseblocks" BB* : term
+
+def bbToIdent : Lean.TSyntax `BB → Lean.TSyntax `ident
+  | `(BB| block $x:ident ($_args,*) {$_cs}) => x
+  | `(BB| block $x:ident ($_args,*) sporks ($_ss) {$_cs}) => x
+  | _ => panic "unknown syntax for basic block"
+
+def elabSSAAtom : Lean.Macro
+  | `(ssa_atom| $n:num) => `(Atom.val ($n))
+  | `(ssa_atom| $x:ident) => `(Atom.var (Var.mk ($x)))
+  | _ => Lean.Macro.throwUnsupported
+
+def elabSSAUop : Lean.Macro
+  | `(ssa_unaop| -) => `(Uop.INEG)
+  | `(ssa_unaop| ¬) => `(Uop.LNOT)
+  | _ => Lean.Macro.throwUnsupported
+
+def elabSSABop : Lean.Macro
+  | `(ssa_binop| +)  => `(Bop.IADD)
+  | `(ssa_binop| -)  => `(Bop.ISUB)
+  | `(ssa_binop| *)  => `(Bop.IMUL)
+  | `(ssa_binop| /)  => `(Bop.IDIV)
+  | `(ssa_binop| %)  => `(Bop.IMOD)
+  | `(ssa_binop| <)  => `(Bop.ILT)
+  | `(ssa_binop| <=) => `(Bop.ILE)
+  | `(ssa_binop| ≤)  => `(Bop.ILE)
+  | `(ssa_binop| >)  => `(Bop.IGT)
+  | `(ssa_binop| >=) => `(Bop.IGE)
+  | `(ssa_binop| ≥)  => `(Bop.IGE)
+  | `(ssa_binop| ==) => `(Bop.IEQ)
+  | `(ssa_binop| !=) => `(Bop.INE)
+  | `(ssa_binop| &&) => `(Bop.LAND)
+  | `(ssa_binop| ||) => `(Bop.LOR)
+  | `(ssa_binop| ^^) => `(Bop.LXOR)
+  | _ => Lean.Macro.throwUnsupported
+
+macro_rules
+  -- if only one element, first try to use that element
+  -- as the list itself, otherwise a singleton
+  -- this parses both list?[1,2,3] and list?[x] for some list x
+  | `(list?[$x:term]) => `(by first | exact [($x)] | exact ($x))
+  | `(list?[$xs,*]) => `([$xs,*])
+
+  | `(goto $b ($args,*)) => `(Cont.mk ($b) list?[$args,*])
+
+  | `(CALL $f ($args,*) ⊳ $cont) => `(Transfer.call ($f) list?[$args,*] ($cont))
+  | `(RETURN ($args,*)) => `(Transfer.retn list?[$args,*])
+  | `(GOTO $b ($args,*)) => `(Transfer.goto (goto $b ($args,*)))
+  | `(SPORK ($body, $f ($args,*) ) ) => `(Transfer.spork ($body) ($f) list?[$args,*])
+  | `(SPOIN ($unpr, $prom)) => `(Transfer.spoin ($unpr) ($prom))
+  | `(IF $cond THEN $tt ELSE $ff) =>
+      elabSSAAtom cond >>= λ cond' =>
+      `(Transfer.ite ($(⟨cond'⟩)) ($tt) ($ff))
+
+  | `(ssa_expr| $a:ssa_atom) =>
+      elabSSAAtom a >>= λ a' =>
+      `(Expr.nop ($(⟨a'⟩)))
+  | `(ssa_expr| $o:ssa_unaop $a:ssa_atom) =>
+      elabSSAUop o >>= λ o' =>
+      elabSSAAtom a >>= λ a' =>
+      `(Expr.uop ($(⟨o'⟩)) ($(⟨a'⟩)))
+  | `(ssa_expr| $a:ssa_atom $o:ssa_binop $b:ssa_atom) =>
+      elabSSABop o >>= λ o' =>
+      elabSSAAtom a >>= λ a' =>
+      elabSSAAtom b >>= λ b' =>
+      `(Expr.bop ($(⟨o'⟩)) ($(⟨a'⟩)) ($(⟨b'⟩)))
+
+  | `([expr| $se:ssa_expr ]) => `($(⟨se.1⟩))
+
+  | `(stmts $_ { $t:term }) => `(Code.trfr ($t))
+  | `(stmts $i { $x:ident ← $t:ssa_expr, $s:stmtget }) =>
+      `(Code.stmt ([expr|$t]) (let $x := Var.mk ($i); stmts $(Lean.Syntax.mkNatLit i.getNat.succ) { $s }))
+
+  | `(countIdents $ids:ident*) =>
+      let n := ids.size
+      return Lean.Syntax.mkNatLit n
+
+  | `(blocklets from $_ in $t) => `($t)
+  | `(blocklets $x:ident $xs:ident* from $i in $t) =>
+      `(let $x := $i; blocklets $xs* from $(Lean.Syntax.mkNatLit i.getNat.succ) in $t)
+
+  | `(func ($bbs,*)) => `(mkfunc (blocklets $(bbs.getElems.map bbToIdent)* from 0 in parseblocks $bbs*))
+  | `(parseblocks) => `([])
+  | `(parseblocks block $x:ident ($args:ident,*) {$cs:stmtget} $bbs:BB*) =>
+      `(Block.mk (BlockSig.mk $(Lean.Syntax.mkNatLit args.getElems.size) []) (blocklets $args* from 0 in stmts 0 {$cs}) :: parseblocks $bbs*)
+  | `(parseblocks block $x:ident ($args:ident,*) sporks ($ss:term,*) {$cs:stmtget} $bbs:BB*) =>
+      `(Block.mk (BlockSig.mk $(Lean.Syntax.mkNatLit args.getElems.size) list?[$ss,*]) (blocklets $args* from 0 in stmts 0 {$cs}) :: parseblocks $bbs*)
